\documentclass[10pt,a4paper]{article}
\usepackage[utf8]{inputenc}
\usepackage{amsmath}
\usepackage{amsfonts}
\usepackage{amssymb}
\title{Homework 2 Solutions}
\date{}
\begin{document}

\maketitle
\begin{enumerate}
\item \begin{enumerate}
\item $y' - y = y^2$ is a separable equation, but it can also be identified as a Bernoulli equation with $n = 2.$ This invites the substitution $y^-1 = v \Leftrightarrow y = 1/v.$ Using the Chain Rule, we find $y' = -v^{-2} v',$ so that the equation is transformed into 
\[ -v' - v = 1,\]
a linear equation! Now either the integrating factor or separation methods apply. For example, using separation yields
\[ v= Ce^{-x} - 1. \]
Finally the solution must be written in the original variables, via the transform $y = 1/v,$ so that 
\[ y = \frac{1}{Ce^{-x} -1} \]
\item This nonlinear, nonseparable equation may be identified as a Bernoulli equation with exponent $n = -2.$ This invites the transformation $v = y^3,$ or upon applying the chain rule, $y' = (1/3) v^{-2/3} v'.$ This transforms the equation into the linear equation 
\[ v' - \frac{6}{x}v = 3x \]
Now we can use the integrating factor method with $\mu = x^{-6}$ to give 
\[ v = -\frac{3}{4}x^2 + Cx^6, \]
and finally 
\[ y = (Cx^6 - \frac{3}{4}x^2 ) ^{1/3}. \]
\item $t^2 y' + 2ty - y^3 = 0$ is a Bernoulli equation with $n = 3.$ The substitution is thus $y^{-2} = v$ and $y' = -(1/2)v^{-3/2}v'.$ Plugging this into the equation reduces it to the linear equation 
\[ v' - \frac{4}{t}v + \frac{2}{t^2} = 0. \]
This can be solved via the integrating factor method, where the integrating factor $\mu = t^{-4}.$ Hence 
\[ v = \frac{2}{5t} + Ct^4 \Rightarrow y = \frac{1}{(2/(5t) + Ct^4)^{1/2}} \]
\end{enumerate}
\item \begin{enumerate}
\item $y' = 1+t^2 - 2ty + y^2$ has the particular solution $y_1(t) = t.$ The Ricatti ansatz $y = t + 1/v$ means $y' = 1-v^{-2}v',$ which is substituted into the equation to reduce it to 
\[ v' = -1 \]
a great simplification. Thus $v = C - t,$ and 
\[ y(t) = t + \frac{1}{C-t}. \]
\item This Ricatti equation has $y_1(t) = 1/t,$ so that 
\[ y' = \frac{-1}{t^2} - \frac{1}{v^2} v' \]
which is plugged in to the equation to give the linear equation 
\[ v' + \frac{v}{t} = -1. \]
This has an integrating factor of $\mu = t,$ so that $v = -t/2 + C/t.$ Finally 
\[ y = \frac{1}{t} + \frac{2t}{C-t^2} \]
after a bit of algebra.
\end{enumerate}
\item \begin{enumerate}
\item Since the equation is homogeneous, $y=0$ is a solution to the IVP $y(0) = 0.$
\item The ODE is nonlinear, so we may separate it to give 
\[ \frac{1}{y^{1/3}}y' = \sin(2t). \]
Subsequently, computing the integrals
\[ \frac{3y^{2/3}}{2}=\frac{1-\cos(2t)}{2} = \sin^2(t), \]
so that the two other solutions to this initial value problem are
\[ y = \pm \sqrt{8/27} \sin^3(t). \]
\item The non-uniqueness may be traced back to the failure of 
\[ \frac{\partial}{\partial y}(y^{1/3} \sin(2t)) \] 
to be continuous at zero, so that the hypotheses of the Existence \& Uniqueness Theorem are not satisfied.
\end{enumerate}
\end{enumerate}


\end{document}